\documentclass[12pt,letterpaper]{article}

\usepackage[margin=1in]{geometry}
\usepackage{fancyhdr}
\usepackage{amsmath}
\pagestyle{fancy}
\rhead{Quaternion Exercise}
\lhead{\textbf{Phien Nguyen}}

\begin{document}
1. What is the Quaternion that would rotate this vector by 90 degrees around the zaxis?
\\
$$
     \begin{aligned}
         q & = cos(45) + 0sin(45)i + 0sin(45)j + 1sin(45)k
         \\
         q & = \frac{\sqrt{2}}{2} + \frac{\sqrt{2}}{2}k
         \\
     \end{aligned}
$$

2. What quaternion would rotate this vector by 90 degrees around the y-axis?
\\
$$
    \begin{aligned}
        q & = cos(45) + 0sin(45)i + 1sin(45)j + 0sin(45)k
        \\
        q & = \frac{\sqrt{2}}{2} + \frac{\sqrt{2}}{2}j
        \\
    \end{aligned}
$$

3. What will we have by rotating vector v using the quaternion in question 1 and then using the quaternion in question 2?
$$
    \begin{aligned}
        v' & = qvq^{-1}
        \\
        & = (\frac{\sqrt{2}}{2} + \frac{\sqrt{2}}{2}k)(2i + 2j)(\frac{\sqrt{2}}{2} - \frac{\sqrt{2}}{2}k)
        \\
        & = (\sqrt{2}i + \sqrt{2}ki + \sqrt{2}j + \sqrt{2}kj)(\frac{\sqrt{2}}{2} - \frac{\sqrt{2}}{2}k)
        \\
        & = 2\sqrt{2}j(\frac{\sqrt{2}}{2} - \frac{\sqrt{2}}{2}k) = 2j - 2jk = 2j -2i
        \\
        v' & = (\frac{\sqrt{2}}{2} + \frac{\sqrt{2}}{2}j)(2j - 2i)(\frac{\sqrt{2}}{2} - \frac{\sqrt{2}}{2}j)
        \\
        & = \sqrt{2}j + \sqrt{2}j^{2} - \sqrt{2}i - \sqrt{2}ji(\frac{\sqrt{2}}{2} - \frac{\sqrt{2}}{2}j)
        \\
        & = 2j + 2k
    \end{aligned}
$$
4. What is the quaternion that achieves the same rotation results by combining quaternion in question 1 and 2? In other words, what quaternion can we use to rotate the vector v to the result of question 3?
$$
    \begin{aligned}
        q & = -\frac{\sqrt{2}}{2} + \frac{\sqrt{2}}{2}j
        \\
        v' & = qvq'
        \\
        & = (-\frac{\sqrt{2}}{2} + \frac{\sqrt{2}}{2}j)(2i + 2j)(-\frac{\sqrt{2}}{2} - \frac{\sqrt{2}}{2}j)
        \\
        & = -\sqrt{2}i + \sqrt{2}ji - \sqrt{2}j + \sqrt{2}j^{2}(-\frac{\sqrt{2}}{2} - \frac{\sqrt{2}}{2}j)
        \\
        & = i + k + j + 1 - ij + jk + j^{2} + j
        \\
        q' & = 2j + 2k
    \end{aligned}
$$

\end{document}
